Lots of semantics fixes and improvements in service of more consistently
using the underlying  type for defining semantics. Structs make this
tricky because two named struct types might have the same underlying
struct literal type (e.g. an empty struct), but they should be treated
separately (e.g. with their own record types). This is now handled by
sealing the field decls of structs and using a new `EqualsUnfold`
typeclass to only unfold where it's useful (e.g. for struct composite
literals).

new/golang/defn/postlang.v
@@ -4,6 +4,12 @@
 From Perennial.goose_lang Require Export lang.
 From Perennial Require Export base.
 
+Class EqualsUnfold {A : Type} (a a' : A) :=
+  { equals_unfold : a = a' }.
+Global Hint Mode EqualsUnfold + + - : typeclass_instances.
+
+Global Notation "a =→ a'" := (EqualsUnfold a a') (at level 70).
+
 #[warning="-uniform-inheritance"]
 Global Coercion GoInstruction : go_instruction >-> val.
 
@@ -100,7 +106,7 @@ Class GoSemanticsFunctions {ext : ffi_syntax} :=
     (* This uses a Gallina [Type] because there are multiple [go.type]s that
        have the same [Type] representation (e.g. uint64/int64, *X/*Y), but
        offsets are only supposed to depend on the Gallina representation. *)
-    is_type_repr : go.type → Type → Prop;
+    TypeRepr : ∀ (t : go.type) (V : Type) `{!ZeroVal V}, Prop;
     struct_field_ref : Type → go_string → loc → loc;
 
     array_index_ref (elem_type : Type) (i : Z) (l : loc) : loc;
@@ -135,7 +141,7 @@ Class MethodUnfold t m (m_impl : val) : Prop :=
 Global Hint Mode MethodUnfold ! ! - : typeclass_instances.
 End unfolding_defs.
 
-Inductive tag := | under | internal | internal_under.
+Inductive tag := | under | under_t (t : go.type) | internal | internal_under.
 
 Module go.
 Section defs.
@@ -255,6 +261,17 @@ Notation "s  ≤u  t" := (UnderlyingEq s t) (at level 70).
 Notation "s  <u  t" := (UnderlyingDirectedEq s t) (at level 70).
 Notation "t  ↓u  tunder" := (IsUnderlying t tunder) (at level 70).
 
+Existing Class TypeRepr.
+Global Hint Mode TypeRepr - - + - - : typeclass_instances.
+
+Class TypeReprUnderlying u V `{!GoSemanticsFunctions} `{!ZeroVal V} : Prop :=
+  { type_repr_underlying_def `{!t ↓u u} : TypeRepr t V }.
+Global Hint Mode TypeReprUnderlying + - - - : typeclass_instances.
+
+Global Instance type_repr_underlying t u V `{!GoSemanticsFunctions} `{!ZeroVal V} :
+  t ↓u u → TypeReprUnderlying u V → TypeRepr t V.
+Proof. intros. eapply type_repr_underlying_def. Qed.
+
 (* Helper definition to cover types for which `a == b` always executes safely. *)
 Class IsStrictlyComparable t V `{!EqDecision V} `{!GoSemanticsFunctions} : Prop :=
   {
@@ -302,18 +319,9 @@ Fixpoint struct_field_type (f : go_string) (fds : list go.field_decl) : go.type 
       else struct_field_type f fds
   end.
 
-Class TypeRepr t V `{!ZeroVal V} `{!GoSemanticsFunctions} : Prop :=
-  {
-    type_repr : is_type_repr t V;
-    #[global] go_zero_val_step :: ⟦GoZeroVal t, #()⟧ ⤳ #(zero_val V);
-  }.
-Global Hint Mode TypeRepr ! - - - : typeclass_instances.
-
 Notation "s  ≤u  t" := (UnderlyingEq s t) (at level 70).
 Notation "s  <u  t" := (UnderlyingDirectedEq s t) (at level 70).
 Notation "t  ↓u  tunder" := (IsUnderlying t tunder) (at level 70).
-
-
 
 Class IntoValUnfold V f :=
   {
@@ -369,6 +377,8 @@ Class CoreSemantics `{!GoSemanticsFunctions} : Prop :=
    ⟦StructFieldSet t_under f, v⟧ ⤳[under] e → ⟦StructFieldSet t f, v⟧ ⤳ e;
   #[global] struct_field_ref_step_underlying `{!t ↓u t_under} f v e ::
     ⟦StructFieldRef t_under f, v⟧ ⤳[under] e → ⟦StructFieldRef t f, v⟧ ⤳ e;
+  #[global] go_zero_val_step_underlying `{!t ↓u t_under} v e ::
+    ⟦GoZeroVal t_under, v⟧ ⤳[under] e → ⟦GoZeroVal t, v⟧ ⤳ e;
 
   #[global] go_func_resolve_step n ts :: ⟦FuncResolve n ts, #()⟧ ⤳ #(functions n ts);
   #[global] go_method_resolve_step m t rcvr `{!t ↓u tunder} `{!NotInterface tunder} ::
@@ -379,7 +389,7 @@ Class CoreSemantics `{!GoSemanticsFunctions} : Prop :=
      panic if the base address is nil. This is a bit of a headache because every
      program step executing [StructFieldRef] will need to have a precondition
      that [l ≠ null]. *)
-  #[global] struct_field_ref_step t f l V `{!ZeroVal V} `{!TypeRepr t V} ::
+  #[global] struct_field_ref_step t f l `{!ZeroVal V} `{!TypeRepr t V} ::
     ⟦StructFieldRef t f, #l⟧ ⤳[under] #(struct_field_ref V f l);
 
   (* The language spec doesn't say anything about the addresses of zero-sized
@@ -403,12 +413,21 @@ Class CoreSemantics `{!GoSemanticsFunctions} : Prop :=
   #[global] into_val_unfold_loc :: IntoValUnfold _ (λ x, LitV $ LitLoc x);
   #[global] into_val_unfold_unit :: IntoValUnfold unit (λ _, LitV LitUnit);
 
-  #[global] type_repr_pointer t :: TypeRepr (go.PointerType t) loc;
-  #[global] type_repr_function sig :: TypeRepr (go.FunctionType sig) func.t;
-  #[global] type_repr_slice elem_type :: TypeRepr (go.SliceType elem_type) slice.t;
-  #[global] type_repr_interface elems :: TypeRepr (go.InterfaceType elems) interface.t;
-  #[global] type_repr_channel dir elem_type :: TypeRepr (go.ChannelType dir elem_type) chan.t;
-  #[global] type_repr_map key_type elem_type :: TypeRepr (go.MapType key_type elem_type) map.t;
+  #[global] go_zero_val_step `{!ZeroVal V} `{!TypeRepr t V} ::
+    ⟦GoZeroVal t, #()⟧ ⤳ #(zero_val V);
+
+  #[global] go_zero_val_pointer t ::
+    TypeReprUnderlying (go.PointerType t) loc;
+  #[global] go_zero_val_function sig ::
+    TypeReprUnderlying (go.FunctionType sig) func.t;
+  #[global] go_zero_val_slice elem_type ::
+    TypeReprUnderlying (go.SliceType elem_type) slice.t;
+  #[global] go_zero_val_interface elems ::
+    TypeReprUnderlying (go.InterfaceType elems) interface.t;
+  #[global] go_zero_val_channel dir elem_type ::
+    TypeReprUnderlying (go.ChannelType dir elem_type) chan.t;
+  #[global] go_zero_val_map key_type elem_type ::
+    TypeReprUnderlying (go.MapType key_type elem_type) map.t;
 
   #[global] core_comparison_sem :: CoreComparisonSemantics;
 
@@ -416,10 +435,10 @@ Class CoreSemantics `{!GoSemanticsFunctions} : Prop :=
     ⟦CompositeLiteral (go.PointerType elem_type), l⟧ ⤳[under]
     GoAlloc elem_type (CompositeLiteral elem_type l);
 
-  #[global] composite_literal_struct l `{!t ↓u (go.StructType fds)} ::
-    ⟦CompositeLiteral t, (LiteralValueV l)⟧ ⤳[under]
+  #[global] composite_literal_struct l `{!fds =→ fds_unsealed} ::
+    ⟦CompositeLiteral (go.StructType fds), (LiteralValueV l)⟧ ⤳[under]
     (match l with
-          | [] => GoZeroVal t #()
+          | [] => GoZeroVal (go.StructType fds) #()
           | KeyedElement None _ :: _ =>
               (* unkeyed struct literal *)
               foldl (λ v '(fd, ke),
@@ -427,19 +446,19 @@ Class CoreSemantics `{!GoSemanticsFunctions} : Prop :=
                          match fd with go.FieldDecl n t | go.EmbeddedField n t => (n, t) end in
                        match ke with
                        | KeyedElement None (ElementExpression from e) =>
-                           StructFieldSet t field_name (v, Convert from field_type e)%E
+                           StructFieldSet (go.StructType fds) field_name (v, Convert from field_type e)%E
                        | _ => Panic "invalid Go code"
                        end
-                ) (GoZeroVal t #()) (zip fds l)
+                ) (GoZeroVal (go.StructType fds) #()) (zip fds_unsealed l)
           | KeyedElement (Some _) _ :: _ =>
               (* keyed struct literal *)
               foldl (λ v ke,
                        match ke with
                        | KeyedElement (Some (KeyField field_name)) (ElementExpression from e) =>
-                           StructFieldSet t field_name (v, Convert from (struct_field_type field_name fds) e)%E
+                           StructFieldSet (go.StructType fds) field_name (v, Convert from (struct_field_type field_name fds_unsealed) e)%E
                        | _ => Panic "invalid Go code"
                        end
-                ) (GoZeroVal t #()) l
+                ) (GoZeroVal (go.StructType fds) #()) l
           end);
 
   #[global] alloc_underlying `[!t ↓u t_under] v e ::
@@ -449,9 +468,9 @@ Class CoreSemantics `{!GoSemanticsFunctions} : Prop :=
   #[global] store_underlying `[!t ↓u t_under] v e ::
     ⟦GoStore t_under, v⟧ ⤳[internal_under] e → ⟦GoStore t, v⟧ ⤳[internal] e;
 
-  #[global] alloc_primitive v t (H : is_primitive t) ::
-    ⟦GoAlloc t, v⟧ ⤳[internal_under] (ref_one v)%E;
-  #[global] alloc_struct v fds ::
+  #[global] alloc_primitive v u (H : is_primitive u) ::
+    ⟦GoAlloc u, v⟧ ⤳[internal_under] (ref_one v)%E;
+  #[global] alloc_struct v `{!fds =→ fds_unsealed} ::
     ⟦GoAlloc (go.StructType fds), v⟧ ⤳[internal_under]
       (let: "l" := GoPrealloc #() in
        foldr (λ fd alloc_rest,
@@ -464,13 +483,13 @@ Class CoreSemantics `{!GoSemanticsFunctions} : Prop :=
                 (if: ("l_field" ≠⟨go.PointerType field_type⟩ field_addr) then AngelicExit #()
                  else #());;
                 alloc_rest
-         ) #() fds ;;
+         ) #() fds_unsealed ;;
        "l")%E;
 
-  #[global] load_primitive t (H : is_primitive t) l ::
-    ⟦GoLoad t, l⟧ ⤳[internal_under] (Read l)%E;
+  #[global] load_primitive u (H : is_primitive u) l ::
+    ⟦GoLoad u, l⟧ ⤳[internal_under] (Read l)%E;
 
-  #[global] load_struct fds l ::
+  #[global] load_struct fds l `{!fds =→ fds_unsealed} ::
     ⟦GoLoad (go.StructType fds), l⟧ ⤳[internal_under]
       (foldl (λ struct_so_far fd,
                 let (field_name, field_type) := match fd with
@@ -480,11 +499,11 @@ Class CoreSemantics `{!GoSemanticsFunctions} : Prop :=
                 let field_addr := StructFieldRef (go.StructType fds) field_name l in
                 let field_val := GoLoad field_type field_addr in
                 StructFieldSet (go.StructType fds) field_name (struct_so_far, field_val)
-         )%E (GoZeroVal (go.StructType fds) #()) fds)%V;
+         )%E (GoZeroVal (go.StructType fds) #()) fds_unsealed)%V;
 
-  #[global] store_primitive t (H : is_primitive t) l v ::
-    ⟦GoStore t, (l, v)⟧ ⤳[internal_under] (l <- v)%E;
-  #[global] store_struct fds l v ::
+  #[global] store_primitive u (H : is_primitive u) l v ::
+    ⟦GoStore u, (l, v)⟧ ⤳[internal_under] (l <- v)%E;
+  #[global] store_struct `{!fds =→ fds_unsealed} l v ::
     ⟦GoStore (go.StructType fds), (l, v)⟧ ⤳[internal_under]
       (foldl (λ store_so_far fd,
                 store_so_far;;
@@ -495,7 +514,7 @@ Class CoreSemantics `{!GoSemanticsFunctions} : Prop :=
                 let field_addr := StructFieldRef (go.StructType fds) field_name l in
                 let field_val := StructFieldGet (go.StructType fds) field_name v in
                 GoStore field_type (field_addr, field_val)
-         )%E (#()) fds)%V;
+         )%E (#()) fds_unsealed)%V;
 
   #[global] is_convert_underlying_same t v :: ⟦Convert t t, v⟧ ⤳[under] v;
   #[global] convert_same t v :: ⟦Convert t t, v⟧ ⤳ v;
