new/golang/defn/loop.v
@@ -1,5 +1,4 @@
 From New.golang.defn Require Export exception.
-From Perennial Require Import base.
 
 Section goose_lang.
 Context {ext : ffi_syntax} {go_gctx : GoGlobalContext}.
