new/golang/theory/array.v
@@ -52,7 +52,7 @@ Proof.
   rewrite seq_S fmap_app /=. f_equal. f_equal. lia.
 Qed.
 
-Context `{!go.TypeRepr t V}.
+Context `{!TypeRepr t V}.
 Global Instance into_val_typed_array n : IntoValTyped (array.t V n) (go.ArrayType n t).
 Proof.
   pose proof go.tagged_steps internal.
